books/centaur/fgl/add-primitives.lisp
@@ -228,6 +228,16 @@
              :atom-alist `((<fn> . ,fn)))
             (fgl-primitive-fncall-entries (cdr table) last)))))
 
+(defun fgl-binder-fncall-entries (table last)
+  (Declare (Xargs :mode :program))
+  (if (atom table)
+      `((otherwise ,last))
+    (b* ((fn (caar table)))
+      (cons (acl2::template-subst
+             '(<fn> (<fn> origfn args interp-st state))
+             :atom-alist `((<fn> . ,fn)))
+            (fgl-binder-fncall-entries (cdr table) last)))))
+
 (defun formula-check-thms (name table)
   (if (atom table)
       nil
@@ -242,7 +252,7 @@
             (formula-check-thms name (cdr table))))))
 
 
-(defun install-fgl-primitives-fn (prefix state)
+(defun install-fgl-metafns-fn (prefix state)
   (declare (xargs :mode :program :stobjs state))
   (b* ((wrld (w state))
        (name-formula-checks (intern-in-package-of-symbol
@@ -271,9 +281,9 @@
           :returns (mv successp ans new-interp-st new-state)
           :ignore-ok t
           (case (pseudo-fnsym-fix primfn)
-            . <entries>) ;;,(fgl-primitive-fncall-entries (table-alist 'fgl-primitives wrld)))
+            . <prim-entries>) ;;,(fgl-primitive-fncall-entries (table-alist 'fgl-primitives wrld)))
           ///
-          <thms>
+          <prim-thms>
           (defret eval-of-<fn>
             (implies (and successp
                           (equal contexts (interp-st->equiv-contexts interp-st))
@@ -295,74 +305,6 @@
                                                 (fgl-object-eval call env (interp-st->logicman interp-st))))))
           (fty::deffixequiv <prefix>-primitive-fncall))
 
-        ;; bozo, dumb theorem needed to prove fixequiv hook
-        (local (defthm pseudo-fnsym-fix-equal-forward
-                 (implies (equal (pseudo-fnsym-fix x) (pseudo-fnsym-fix y))
-                          (pseudo-fnsym-equiv x y))
-                 :rule-classes :forward-chaining))
-
-        (defattach
-          ;; BOZO add all these back in as well as substitutions for -concretize functions
-          ;; if we support adding new evaluators.
-          ;; (fgl-ev <prefix>-ev)
-          ;; (fgl-ev-list <prefix>-ev-list)
-          ;; (fgl-apply <prefix>-apply :attach nil)
-          ;; (fgl-object-eval-fn <prefix>-object-eval-fn :attach nil)
-          ;; (fgl-objectlist-eval-fn <prefix>-objectlist-eval-fn :attach nil)
-          ;; (fgl-object-alist-eval-fn <prefix>-object-alist-eval-fn :attach nil)
-          ;; (fgl-ev-falsify <prefix>-ev-falsify :attach nil)
-          ;; (fgl-ev-meta-extract-global-badguy <prefix>-ev-meta-extract-global-badguy :attach nil)
-          (fgl-primitive-fncall-stub <prefix>-primitive-fncall)
-          (fgl-primitive-formula-checks-stub <prefix>-formula-checks)
-          :hints(("Goal"
-                  :do-not '(preprocess simplify)
-                  :clause-processor dumb-clausify-cp)
-                 (let ((term (car (last clause))))
-                   (case-match term
-                     (('equal (fn . &) . &)
-                      `(:clause-processor (beta-reduce-by-hint-cp clause ',fn state)
-                        :do-not nil))
-                     (& (cond ((member-atoms '<prefix>-primitive-fncall term)
-                               '(:do-not nil))
-                              (t '(:do-not nil)))))))
-          ))
-     :str-alist `(("<PREFIX>" ,(symbol-name prefix) . ,prefix))
-     :atom-alist `(;; (<all-formulas> . ,all-formulas)
-                   ;; (<formula-check-thms> . ,formula-check-thms)
-                   (<entries> . ,(fgl-primitive-fncall-entries (table-alist 'fgl-primitives wrld) '(mv nil nil interp-st state)))
-                   ;; (<all-formulas> . ,all-formulas)
-                   (<formula-check-thms> . ,formula-check-thms)
-                   (<formula-check-fns> . ,formula-check-fns))
-     :splice-alist `((<thms> . ,*fgl-primitive-rule-thms*)))
-    
-    ))
-
-(defmacro install-fgl-primitives (name)
-  `(make-event
-    (install-fgl-primitives-fn ',name state)))
-
-
-(defun install-fgl-metafns-fn (prefix state)
-  (declare (xargs :mode :program :stobjs state))
-  (b* ((wrld (w state))
-       (name-formula-checks (intern-in-package-of-symbol
-                             (concatenate 'string (symbol-name prefix) "-FORMULA-CHECKS")
-                             prefix))
-       (formula-checks-table (table-alist 'fgl-formula-checks wrld))
-       (formula-check-fns (set::mergesort (append-alist-vals formula-checks-table)))
-       (formula-check-thms (formula-check-thms name-formula-checks formula-checks-table))
-       )
-    (acl2::template-subst
-     '(progn
-        ;; (def-fgl-object-eval <prefix> nil :union-previous t)
-        (cmr::def-formula-checker <prefix>-formula-checks <formula-check-fns>)
-        (progn . <formula-check-thms>)
-
-        ;; (make-event
-        ;;  (cons 'progn
-        ;;        (instantiate-fgl-primitive-correctness-thms-fn
-        ;;         (table-alist 'fgl-primitives (w state)))))
-
         (define <prefix>-meta-fncall ((metafn pseudo-fnsym-p)
                                       (call fgl-object-p)
                                       (interp-st interp-st-bfrs-ok)
@@ -371,9 +313,9 @@
           :returns (mv successp rhs bindings new-interp-st new-state)
           :ignore-ok t
           (case (pseudo-fnsym-fix metafn)
-            . <entries>) ;;,(fgl-primitive-fncall-entries (table-alist 'fgl-primitives wrld)))
+            . <meta-entries>) ;;,(fgl-primitive-fncall-entries (table-alist 'fgl-primitives wrld)))
           ///
-          <thms>
+          <meta-thms>
           (defret eval-of-<fn>
             (implies (and successp
                           (equal contexts (interp-st->equiv-contexts interp-st))
@@ -396,6 +338,47 @@
                       (fgl-object-bindings-eval bindings env (interp-st->logicman new-interp-st)))))
           (fty::deffixequiv <prefix>-meta-fncall))
 
+        (define <prefix>-binder-fncall ((bindfn pseudo-fnsym-p)
+                                        (origfn pseudo-fnsym-p)
+                                        (args fgl-objectlist-p)
+                                        (interp-st interp-st-bfrs-ok)
+                                        state)
+          :guard (interp-st-bfr-listp (fgl-objectlist-bfrlist args))
+          :returns (mv successp rhs bindings rhs-contexts new-interp-st new-state)
+          :ignore-ok t
+          (case (pseudo-fnsym-fix bindfn)
+            . <bind-entries>) ;;,(fgl-primitive-fncall-entries (table-alist 'fgl-primitives wrld)))
+          ///
+          <bind-thms>
+          (defret eval-of-<fn>
+            (implies (and successp
+                          (equal contexts (interp-st->equiv-contexts interp-st))
+                          (fgl-ev-meta-extract-global-facts :state st)
+                          ;; (,name-formula-checks st)
+                          (<prefix>-formula-checks st)
+                          (equal (w st) (w state))
+                          (interp-st-bfrs-ok interp-st)
+                          (interp-st-bfr-listp (fgl-objectlist-bfrlist args))
+                          (logicman-pathcond-eval (fgl-env->bfr-vals env)
+                                                  (interp-st->constraint interp-st)
+                                                  (interp-st->logicman interp-st))
+                          (logicman-pathcond-eval (fgl-env->bfr-vals env)
+                                                  (interp-st->pathcond interp-st)
+                                                  (interp-st->logicman interp-st))
+                          (fgl-ev-context-equiv-forall-extensions
+                           rhs-contexts
+                           var-val
+                           rhs (fgl-object-bindings-eval bindings env (interp-st->logicman new-interp-st))))
+                     (equal (fgl-ev-context-fix contexts (fgl-ev (cons origfn
+                                                                       (cons (list 'quote var-val)
+                                                                             (kwote-lst
+                                                                              (fgl-objectlist-eval
+                                                                               args env
+                                                                               (interp-st->logicman interp-st)))))
+                                                           nil))
+                      (fgl-ev-context-fix contexts var-val))))
+          (fty::deffixequiv <prefix>-binder-fncall))
+
         ;; bozo, dumb theorem needed to prove fixequiv hook
         (local (defthm pseudo-fnsym-fix-equal-forward
                  (implies (equal (pseudo-fnsym-fix x) (pseudo-fnsym-fix y))
@@ -413,8 +396,10 @@
           ;; (fgl-object-alist-eval-fn <prefix>-object-alist-eval-fn :attach nil)
           ;; (fgl-ev-falsify <prefix>-ev-falsify :attach nil)
           ;; (fgl-ev-meta-extract-global-badguy <prefix>-ev-meta-extract-global-badguy :attach nil)
+          (fgl-primitive-fncall-stub <prefix>-primitive-fncall)
           (fgl-meta-fncall-stub <prefix>-meta-fncall)
-          (fgl-meta-formula-checks-stub <prefix>-formula-checks)
+          (fgl-binder-fncall-stub <prefix>-binder-fncall)
+          (fgl-formula-checks-stub <prefix>-formula-checks)
           :hints(("Goal"
                   :do-not '(preprocess simplify)
                   :clause-processor dumb-clausify-cp)
@@ -423,23 +408,29 @@
                      (('equal (fn . &) . &)
                       `(:clause-processor (beta-reduce-by-hint-cp clause ',fn state)
                         :do-not nil))
-                     (& (cond ((member-atoms '<prefix>-meta-fncall term)
-                               '(:do-not nil))
+                     (& (cond ;; ((member-atoms '<prefix>-primitive-fncall term)
+                              ;;  '(:do-not nil))
                               (t '(:do-not nil)))))))
           ))
      :str-alist `(("<PREFIX>" ,(symbol-name prefix) . ,prefix))
      :atom-alist `(;; (<all-formulas> . ,all-formulas)
                    ;; (<formula-check-thms> . ,formula-check-thms)
-                   (<entries> . ,(fgl-primitive-fncall-entries (table-alist 'fgl-metafns wrld) '(mv nil nil nil interp-st state)))
+                   (<prim-entries> . ,(fgl-primitive-fncall-entries (table-alist 'fgl-primitives wrld) '(mv nil nil interp-st state)))
+                   (<meta-entries> . ,(fgl-primitive-fncall-entries (table-alist 'fgl-metafns wrld) '(mv nil nil nil interp-st state)))
+                   (<bind-entries> . ,(fgl-binder-fncall-entries (table-alist 'fgl-binderfns wrld)
+                                                                 '(mv nil nil nil nil interp-st state)))
                    ;; (<all-formulas> . ,all-formulas)
                    (<formula-check-thms> . ,formula-check-thms)
                    (<formula-check-fns> . ,formula-check-fns))
-     :splice-alist `((<thms> . ,*fgl-meta-rule-thms*)))
+     :splice-alist `((<prim-thms> . ,*fgl-primitive-rule-thms*)
+                     (<meta-thms> . ,*fgl-meta-rule-thms*)
+                     (<bind-thms> . ,*fgl-binder-rule-thms*)))
     
     ))
 
 (defmacro install-fgl-metafns (name)
   `(make-event
     (install-fgl-metafns-fn ',name state)))
+
 
 
